Prefix: owl: <http://www.w3.org/2002/07/owl#>
Prefix: rdf: <http://www.w3.org/1999/02/22-rdf-syntax-ns#>
Prefix: xsd: <http://www.w3.org/2001/XMLSchema#>
Prefix: rdfs: <http://www.w3.org/2000/01/rdf-schema#>
Prefix: skos: <http://www.w3.org/2004/02/skos/core#>
Prefix: ontolex: <http://www.w3.org/ns/ontolex#>
Prefix: semio: <http://www.ontologydesignpatterns.org/cp/owl/semiotics.owl#>

Ontology: <http://www.w3.org/ns/ontolex#>
Import: <http://www.w3.org/2004/02/skos/core>
Import: <http://www.ontologydesignpatterns.org/cp/owl/semiotics.owl>

# Required to read in Protege
ObjectProperty: semio:denotes
ObjectProperty: semio:hasInterpretant
ObjectProperty: semio:isConceptualizationOf
ObjectProperty: semio:hasConceptualization

ObjectProperty: ontolex:contains
    Annotations: 
        rdfs:comment "The relation between a collection of senses and one particular sense included in it."@en

    Domain: 
        ontolex:LexicalConcept

    Range: 
        ontolex:LexicalSense
    
ObjectProperty: ontolex:isContainedBy
    InverseOf: ontolex:contains

ObjectProperty: ontolex:canonicalForm

    Annotations: 
        rdfs:comment "Indicates the canonical form used to index this lexical lexicalEntry"@en
    
    SubPropertyOf: 
        ontolex:lexicalForm
    
    Characteristics: 
        Functional
    
    Domain: 
        ontolex:LexicalEntry
    
    Range: 
        ontolex:Form
    
    
ObjectProperty: ontolex:reference

    Annotations: 
        rdfs:comment "The relation between the lexical sense of a lexical lexicalEntry and the ontological predicate that represents the denotation."@en
    
    SubPropertyOf:
        semio:isConceptualizationOf

    Characteristics: 
        Functional
    
    Domain: 
        ontolex:LexicalSense
    
ObjectProperty: ontolex:isReferenceOf
    InverseOf: ontolex:reference
    
ObjectProperty: ontolex:sense

    Annotations: 
        rdfs:comment "The relation between a lexical lexicalEntry and on of its lexical senses."@en
        
    SubPropertyOf:
        semio:hasInterpretant

    Domain: 
        ontolex:LexicalEntry
    
    Range: 
        ontolex:LexicalSense
    
ObjectProperty: ontolex:isSenseOf
    InverseOf: ontolex:sense

ObjectProperty: ontolex:otherForm

    Annotations: 
        rdfs:comment "Indicates a variant form of an lexicalEntry"@en
    
    SubPropertyOf: 
        ontolex:lexicalForm
    
    Domain: 
        ontolex:LexicalEntry
    
    Range: 
        ontolex:Form
    
    
ObjectProperty: ontolex:denotes

    Annotations: 
        rdfs:comment "The relation between a lexical lexicalEntry and the logical predicate in an ontology that represents its meaning and has some denotational / model-theoretic semantics."

    EquivalentTo:
        semio:denotes

    SubPropertyChain: 
        ontolex:sense o ontolex:reference
    
    Characteristics: 
        Functional
    
    Domain: 
        ontolex:LexicalEntry
    
ObjectProperty: ontolex:isDenotedBy
    InverseOf: ontolex:denotes    

ObjectProperty: ontolex:concept

    Annotations: 
        rdfs:comment "The relation between an ontology entity and the lexical concept that it corresponds to."@en

    SubPropertyOf:
        semio:hasConceptualization    

    Range:
        ontolex:LexicalConcept
    
ObjectProperty: ontolex:isConceptOf
    InverseOf: ontolex:concept
    
ObjectProperty: ontolex:lexicalEntry

    Annotations: 
        rdfs:comment "Indicates that an lexicalEntry belongs to a lexicon"@en
    
    Domain: 
        ontolex:Lexicon
    
    Range: 
        ontolex:LexicalEntry
        
ObjectProperty: ontolex:isEntryOf
    InverseOf: ontolex:lexicalEntry

ObjectProperty: ontolex:lexicalForm

    Annotations: 
        rdfs:comment "Indicate a single form of an lexicalEntry"@en
    
    Domain: 
        ontolex:LexicalEntry
    
    Range: 
        ontolex:Form
    
    
ObjectProperty: ontolex:evokes

    Annotations: 
        rdfs:comment "The relation between a lexical lexicalEntry and the mental concept that comes to the mind of an agent when reading or hearing the lexicalEntry."@en
        
    SubPropertyOf:
        semio:hasInterpretant

    SubPropertyChain: 
        ontolex:sense o  inverse (ontolex:contains)
    
    Domain: 
        ontolex:LexicalEntry
    
    Range: 
        ontolex:LexicalConcept
    
ObjectProperty: ontolex:isEvokedBy
    InverseOf: ontolex:evokes
    
DataProperty: ontolex:writtenRep

    Annotations: 
        rdfs:comment "Indicates the written representation of a form"@en
    
    Domain: 
        ontolex:Form
    
    
DataProperty: ontolex:language

    Annotations: 
        rdfs:comment "Indicates the language of a lexicon or lexical lexicalEntry, encoded as an ISO-639 code"@en
    
    Domain: 
        ontolex:LexicalEntry
         or ontolex:Lexicon
    
    Range: 
        xsd:string
    
    
# Required to read in Protege
Class: semio:Expression    
Class: semio:Meaning
Class: skos:Concept
Datatype: rdfs:Literal

Class: ontolex:LexicalConcept

    Annotations: 
        rdfs:comment "A  language-specific collection of senses that have a common meaning."@en
    
    SubClassOf: 
        skos:Concept,
        semio:Meaning
    
    DisjointWith: 
        ontolex:Lexicon, ontolex:LexicalEntry, ontolex:Form, ontolex:LexicalSense

    
Class: ontolex:Lexicon

    Annotations: 
        rdfs:comment "The lexicon represents a collection of entries describing the vocabular used by an ontology"@en
    
    SubClassOf: 
        ontolex:language min 1 rdfs:Literal
    
    DisjointWith: 
        ontolex:LexicalConcept, ontolex:LexicalEntry, ontolex:Form, ontolex:LexicalSense
    
Class: ontolex:LexicalEntry

    Annotations: 
        rdfs:comment "A single unit of analysis in the lexicon, i.e. a collection of morphologically related forms, all of which denote the same concept(s)."@en
    
    SubClassOf: 
        semio:Expression
    
    DisjointWith: 
        ontolex:LexicalConcept, ontolex:Lexicon, ontolex:Form, ontolex:LexicalSense
            
Class: ontolex:Form

    Annotations: 
        rdfs:comment "The form represents a single inflected unit of a lexical lexicalEntry with a single pronunciation, although potentially many orthographies"@en
    
    DisjointWith: 
        ontolex:LexicalConcept, ontolex:LexicalEntry, ontolex:Lexicon, ontolex:LexicalSense
    
    
Class: ontolex:LexicalSense

    Annotations: 
        rdfs:comment "A language-specific meaning of a lexical lexicalEntry which abstracts from specific occurrences of the lemma. This class is a lexical sense as it represents a sense of a lexical item."@en
    
    SubClassOf: 
        semio:Meaning
    
    DisjointWith: 
        ontolex:LexicalConcept, ontolex:Lexicon, ontolex:LexicalEntry, ontolex:Form